move the reduction control of the proofmode to its own file and tweak it
* move PROP-envs definitions to environments.v so that we can control them without pulling in coq_tactics
* use reduction-controlled `pm_default` for proofmode accessors

theories/proofmode/coq_tactics.v
@@ -7,140 +7,7 @@ Import env_notations.
 
 Local Notation "b1 && b2" := (if b1 then b2 else false) : bool_scope.
 
-Record envs (PROP : bi) :=
-  Envs { env_intuitionistic : env PROP; env_spatial : env PROP; env_counter : positive }.
-Add Printing Constructor envs.
-Arguments Envs {_} _ _ _.
-Arguments env_intuitionistic {_} _.
-Arguments env_spatial {_} _.
-Arguments env_counter {_} _.
-
-Record envs_wf {PROP} (Δ : envs PROP) := {
-  env_intuitionistic_valid : env_wf (env_intuitionistic Δ);
-  env_spatial_valid : env_wf (env_spatial Δ);
-  envs_disjoint i : env_intuitionistic Δ !! i = None ∨ env_spatial Δ !! i = None
-}.
-
-Definition of_envs {PROP} (Δ : envs PROP) : PROP :=
-  (⌜envs_wf Δ⌝ ∧ □ [∧] env_intuitionistic Δ ∗ [∗] env_spatial Δ)%I.
-Instance: Params (@of_envs) 1.
-Arguments of_envs : simpl never.
-
-(* We seal [envs_entails], so that it does not get unfolded by the
-   proofmode's own tactics, such as [iIntros (?)]. *)
-Definition envs_entails_aux : seal (λ PROP (Δ : envs PROP) (Q : PROP), (of_envs Δ ⊢ Q)).
-Proof. by eexists. Qed.
-Definition envs_entails := envs_entails_aux.(unseal).
-Definition envs_entails_eq : envs_entails = _ := envs_entails_aux.(seal_eq).
-Arguments envs_entails {PROP} Δ Q%I : rename.
-Instance: Params (@envs_entails) 1.
-
-Record envs_Forall2 {PROP : bi} (R : relation PROP) (Δ1 Δ2 : envs PROP) := {
-  env_intuitionistic_Forall2 : env_Forall2 R (env_intuitionistic Δ1) (env_intuitionistic Δ2);
-  env_spatial_Forall2 : env_Forall2 R (env_spatial Δ1) (env_spatial Δ2)
-}.
-
-Definition envs_dom {PROP} (Δ : envs PROP) : list ident :=
-  env_dom (env_intuitionistic Δ) ++ env_dom (env_spatial Δ).
-
-Definition envs_lookup {PROP} (i : ident) (Δ : envs PROP) : option (bool * PROP) :=
-  let (Γp,Γs,n) := Δ in
-  match env_lookup i Γp with
-  | Some P => Some (true, P)
-  | None => P ← env_lookup i Γs; Some (false, P)
-  end.
-
-Definition envs_delete {PROP} (remove_persistent : bool)
-    (i : ident) (p : bool) (Δ : envs PROP) : envs PROP :=
-  let (Γp,Γs,n) := Δ in
-  match p with
-  | true => Envs (if remove_persistent then env_delete i Γp else Γp) Γs n
-  | false => Envs Γp (env_delete i Γs) n
-  end.
-
-Definition envs_lookup_delete {PROP} (remove_persistent : bool)
-    (i : ident) (Δ : envs PROP) : option (bool * PROP * envs PROP) :=
-  let (Γp,Γs,n) := Δ in
-  match env_lookup_delete i Γp with
-  | Some (P,Γp') => Some (true, P, Envs (if remove_persistent then Γp' else Γp) Γs n)
-  | None => ''(P,Γs') ← env_lookup_delete i Γs; Some (false, P, Envs Γp Γs' n)
-  end.
-
-Fixpoint envs_lookup_delete_list {PROP} (remove_persistent : bool)
-    (js : list ident) (Δ : envs PROP) : option (bool * list PROP * envs PROP) :=
-  match js with
-  | [] => Some (true, [], Δ)
-  | j :: js =>
-     ''(p,P,Δ') ← envs_lookup_delete remove_persistent j Δ;
-     ''(q,Hs,Δ'') ← envs_lookup_delete_list remove_persistent js Δ';
-     Some ((p:bool) && q, P :: Hs, Δ'')
-  end.
-
-Definition envs_snoc {PROP} (Δ : envs PROP)
-    (p : bool) (j : ident) (P : PROP) : envs PROP :=
-  let (Γp,Γs,n) := Δ in
-  if p then Envs (Esnoc Γp j P) Γs n else Envs Γp (Esnoc Γs j P) n.
-
-Definition envs_app {PROP : bi} (p : bool)
-    (Γ : env PROP) (Δ : envs PROP) : option (envs PROP) :=
-  let (Γp,Γs,n) := Δ in
-  match p with
-  | true => _ ← env_app Γ Γs; Γp' ← env_app Γ Γp; Some (Envs Γp' Γs n)
-  | false => _ ← env_app Γ Γp; Γs' ← env_app Γ Γs; Some (Envs Γp Γs' n)
-  end.
-
-Definition envs_simple_replace {PROP : bi} (i : ident) (p : bool)
-    (Γ : env PROP) (Δ : envs PROP) : option (envs PROP) :=
-  let (Γp,Γs,n) := Δ in
-  match p with
-  | true => _ ← env_app Γ Γs; Γp' ← env_replace i Γ Γp; Some (Envs Γp' Γs n)
-  | false => _ ← env_app Γ Γp; Γs' ← env_replace i Γ Γs; Some (Envs Γp Γs' n)
-  end.
-
-Definition envs_replace {PROP : bi} (i : ident) (p q : bool)
-    (Γ : env PROP) (Δ : envs PROP) : option (envs PROP) :=
-  if Bool.eqb p q then envs_simple_replace i p Γ Δ
-  else envs_app q Γ (envs_delete true i p Δ).
-
-Definition env_spatial_is_nil {PROP} (Δ : envs PROP) : bool :=
-  if env_spatial Δ is Enil then true else false.
-
-Definition envs_clear_spatial {PROP} (Δ : envs PROP) : envs PROP :=
-  Envs (env_intuitionistic Δ) Enil (env_counter Δ).
-
-Definition envs_clear_persistent {PROP} (Δ : envs PROP) : envs PROP :=
-  Envs Enil (env_spatial Δ) (env_counter Δ).
-
-Definition envs_incr_counter {PROP} (Δ : envs PROP) : envs PROP :=
-  Envs (env_intuitionistic Δ) (env_spatial Δ) (Pos.succ (env_counter Δ)).
-
-Fixpoint envs_split_go {PROP}
-    (js : list ident) (Δ1 Δ2 : envs PROP) : option (envs PROP * envs PROP) :=
-  match js with
-  | [] => Some (Δ1, Δ2)
-  | j :: js =>
-     ''(p,P,Δ1') ← envs_lookup_delete true j Δ1;
-     if p : bool then envs_split_go js Δ1 Δ2 else
-     envs_split_go js Δ1' (envs_snoc Δ2 false j P)
-  end.
-(* if [d = Right] then [result = (remaining hyps, hyps named js)] and
-   if [d = Left] then [result = (hyps named js, remaining hyps)] *)
-Definition envs_split {PROP} (d : direction)
-    (js : list ident) (Δ : envs PROP) : option (envs PROP * envs PROP) :=
-  ''(Δ1,Δ2) ← envs_split_go js Δ (envs_clear_spatial Δ);
-  if d is Right then Some (Δ1,Δ2) else Some (Δ2,Δ1).
-
-Definition prop_of_env {PROP : bi} (Γ : env PROP) : PROP :=
-  let fix aux Γ acc :=
-    match Γ with Enil => acc | Esnoc Γ _ P => aux Γ (P ∗ acc)%I end
-  in
-  match Γ with Enil => emp%I | Esnoc Γ _ P => aux Γ P end.
-
-Definition maybe_wand {PROP : bi} (mP : option PROP) (Q : PROP) : PROP :=
-  match mP with
-  | None => Q
-  | Some P => (P -∗ Q)%I
-  end.
+Notation pm_maybe_wand mP Q := (pm_from_option (λ P, P -∗ Q)%I Q%I mP).
 
 (* Coq versions of the tactics *)
 Section bi_tactics.
@@ -343,7 +210,7 @@ Lemma envs_replace_sound' Δ Δ' i p q Γ :
   envs_replace i p q Γ Δ = Some Δ' →
   of_envs (envs_delete true i p Δ) ⊢ (if q then □ [∧] Γ else [∗] Γ) -∗ of_envs Δ'.
 Proof.
-  rewrite /envs_replace; destruct (Bool.eqb _ _) eqn:Hpq.
+  rewrite /envs_replace; destruct (beq _ _) eqn:Hpq.
   - apply eqb_prop in Hpq as ->. apply envs_simple_replace_sound'.
   - apply envs_app_sound.
 Qed.
@@ -449,8 +316,8 @@ Proof.
   - rewrite /= IH (comm _ Q _) assoc. done.
 Qed.
 
-Lemma maybe_wand_sound (mP : option PROP) Q :
-  maybe_wand mP Q ⊣⊢ (default emp mP -∗ Q).
+Lemma pm_maybe_wand_sound mP Q :
+  pm_maybe_wand mP Q ⊣⊢ (default emp mP -∗ Q).
 Proof. destruct mP; simpl; first done. rewrite emp_wand //. Qed.
 
 Global Instance envs_Forall2_refl (R : relation PROP) :
@@ -751,7 +618,6 @@ Proof.
   rewrite envs_lookup_sound // envs_split_sound //.
   rewrite (envs_app_singleton_sound Δ2) //; simpl.
   rewrite HP1 into_wand /= -(add_modal P1' P1 Q). cancel [P1'].
-
   apply wand_intro_l. by rewrite assoc !wand_elim_r.
 Qed.
 
@@ -1109,7 +975,10 @@ Lemma tac_inv_elim {X : Type} Δ Δ' i j φ p Pinv Pin Pout (Pclose : option (X 
   φ →
   (∀ R, ∃ Δ'',
     envs_app false (Esnoc Enil j
-            (Pin -∗ (∀ x, Pout x -∗ from_option (λ Pclose, Pclose x -∗ Q' x) (Q' x) Pclose) -∗ R)%I) Δ'
+      (Pin -∗
+       (∀ x, Pout x -∗ pm_maybe_wand (pm_option_fun Pclose x) (Q' x)) -∗
+       R
+      )%I) Δ'
       = Some Δ'' ∧
     envs_entails Δ'' R) →
   envs_entails Δ Q.
