theories/proofmode/reduction.v
@@ -1,0 +1,24 @@
+From iris.bi Require Import bi.
+From iris.proofmode Require Import base environments.
+
+Declare Reduction pm_cbv := cbv [
+  (* base *)
+  pm_option_bind pm_from_option pm_option_fun
+  base.beq base.ascii_beq base.string_beq base.positive_beq base.ident_beq
+  (* environments *)
+  env_lookup env_lookup_delete env_delete env_app env_replace
+  env_dom env_intuitionistic env_spatial env_counter env_spatial_is_nil envs_dom
+  envs_lookup envs_lookup_delete envs_delete envs_snoc envs_app
+  envs_simple_replace envs_replace envs_split
+  envs_clear_spatial envs_clear_persistent envs_incr_counter
+  envs_split_go envs_split prop_of_env
+  (* other modules. TODO: we should probably make copies of these,
+     but what will that break? *)
+  Pos.succ
+].
+Ltac pm_eval t :=
+  let u := eval pm_cbv in t in
+  u.
+Ltac pm_reduce :=
+  match goal with |- ?u => let v := pm_eval u in change v end.
+Ltac pm_reflexivity := pm_reduce; exact eq_refl.
